Chase_Lev.thy
@@ -62,31 +62,239 @@ section \<open>Example\<close>
 definition steal
   where "steal v = {(A,A'). A = v#A'}"
 
+definition steal_any
+  where "steal_any = {(A,A'). \<exists>v. A = v#A'}"
+
 definition put
   where "put v = {(A,A'). A' = A@[v]}"
 
-lemma test1[simp]:
-  "st (m(l :=\<^sub>s e)) f = (if l = f then e else st m f)"
-  "rg (m(l :=\<^sub>s e)) r = rg m r"
-  "rg (m(r :=\<^sub>r e)) f = (if f = r then e else rg m f)"
-  by (auto simp: st_upd_def rg_upd_def)
+fun chain
+  where "chain [] Q = Q" | "chain (a#xs) Q = chain xs (wpre a Q)"
+declare chain.simps [simp del]
 
-lemma test2[simp]:
-  "st (m(aux: a)) e = st m e"
-  by (auto simp: aux_upd_def)
+lemma chain_singleI:
+  "wpre a Q = chain [a] Q"
+  unfolding chain.simps by auto
 
-lemma chase_lev_push:
+lemma chain_singleI':
+  "stabilize R Q = chain [env R] Q"
+  unfolding chain.simps by auto
+
+
+lemma chain_lastE:
+  "chain (xs @ [a]) Q = wpre a ( (chain xs Q))"
+  by (induct xs arbitrary: Q) (auto simp: chain.simps)
+
+lemma chain_lastI:
+  "chain [a] (chain xs Q) = chain (xs@[a]) Q"
+  by (induct xs) (auto simp: chain_lastE chain.simps)
+
+lemma stabilize_mono:
+  "P \<turnstile>\<^sub>p Q \<Longrightarrow> stabilize R P  \<turnstile>\<^sub>p stabilize R Q"
+  unfolding stabilize_def pred_defs by auto
+
+lemma pre_mono:
+  "P \<turnstile>\<^sub>p Q \<Longrightarrow> wpre a P \<turnstile>\<^sub>p wpre a Q"
+  by (cases a) (auto intro: stabilize_mono simp: pred_defs)
+
+lemma chain_mono:
+  "P \<turnstile>\<^sub>p Q \<Longrightarrow> chain xs P \<turnstile>\<^sub>p chain xs Q"
+  by (induct xs arbitrary: P Q) (auto simp: pre_mono stabilize_mono chain.simps)
+
+lemma chain1_wpre:
+  "P \<turnstile>\<^sub>p chain xs (wpre a Q) \<Longrightarrow> P \<turnstile>\<^sub>p chain (a#xs) Q"
+  unfolding chain.simps .
+
+lemma chain1_stab:
+  "P \<turnstile>\<^sub>p chain xs (stabilize R Q) \<Longrightarrow> P \<turnstile>\<^sub>p chain (env R#xs) Q"
+  unfolding chain.simps by auto
+
+lemma chain0:
+  "P \<turnstile>\<^sub>p Q \<Longrightarrow> P \<turnstile>\<^sub>p  chain [] Q"
+  unfolding chain.simps .
+
+lemma trans_flip: "\<And>a b c. b \<turnstile>\<^sub>p c \<Longrightarrow> a \<turnstile>\<^sub>p b \<Longrightarrow> a \<turnstile>\<^sub>p c"
+  by (auto simp: pred_defs)
+
+lemma chain1_full:
+  assumes "Q' \<turnstile>\<^sub>p wpre a P"
+  assumes "Q'' \<turnstile>\<^sub>p chain xs Q'"
+  shows "Q'' \<turnstile>\<^sub>p chain (a#xs) P"
+  apply (rule chain1_wpre)
+  apply (rule trans_flip)
+  apply (rule chain_mono)
+  apply (rule trans_flip)
+  apply (rule pre_mono)
+  using assms by auto
+
+lemma chain_extend:
+  "P \<turnstile>\<^sub>p chain xs (Q \<and>\<^sub>p X) \<Longrightarrow> P \<turnstile>\<^sub>p chain xs Q"
+  using chain_mono[of "Q \<and>\<^sub>p X" Q] by (auto simp: pred_defs)
+
+lemma chain_rewrite:
+  "X \<turnstile>\<^sub>p Q \<Longrightarrow> P \<turnstile>\<^sub>p chain xs X \<Longrightarrow> P \<turnstile>\<^sub>p chain xs Q"
+  using chain_mono unfolding pred_defs by blast
+
+definition str where
+  "str R P \<equiv> if stabilize R P = P then P else True\<^sub>p"
+
+lemma str_mono:
+  "Q \<turnstile>\<^sub>p P \<Longrightarrow> Q \<turnstile>\<^sub>p str R P"
+  unfolding str_def by (auto simp: pred_defs)
+
+subsection \<open>Trivial Cases\<close>
+
+named_theorems trivial_thms
+declare subset_UNIV [trivial_thms]
+
+lemma [trivial_thms]: "stabilize R True\<^sub>p = True\<^sub>p"
+  unfolding stabilize_def by simp
+
+lemma [trivial_thms]: "wpre a True\<^sub>p = True\<^sub>p"
+  by (cases a) (auto simp:)
+
+lemma [trivial_thms]:
+  "chain xs True\<^sub>p = True\<^sub>p"
+  by (induct xs) (auto simp: trivial_thms chain.simps)
+
+lemma stabilize_univ:
+  "True\<^sub>p \<turnstile>\<^sub>p stabilize R True\<^sub>p"
+  unfolding stabilize_def by auto
+
+lemma stabilize_str:
+  "str R P \<turnstile>\<^sub>p stabilize R (str R P)"
+  unfolding str_def stabilize_def by simp
+
+lemma stabilize_trivial:
+  "\<forall>m m'. P m \<longrightarrow> R (glb m, glb m') \<longrightarrow> rg m' = rg m \<longrightarrow> P m' \<Longrightarrow> str R P \<turnstile>\<^sub>p stabilize R P"
+  apply (subgoal_tac "str R (P \<and>\<^sub>p True\<^sub>p) \<turnstile>\<^sub>p stabilize R (P)")
+  apply simp
+  sorry
+
+method stabilize_trivial_tac = (rule order_antisym; clarsimp)
+
+method pre_tac =
+  (match conclusion in "Q \<subseteq> pre \<alpha> UNIV" for \<alpha> S Q \<Rightarrow> \<open>succeed\<close>, rule pre_univ) |
+  (match conclusion in "Q \<subseteq> pre \<alpha> (str R P)" for \<alpha> S Q R P \<Rightarrow> \<open>succeed\<close>, pre_str_tac) |
+  (match conclusion in "Q \<subseteq> pre \<alpha> P" for Q \<alpha> S P \<Rightarrow> \<open>succeed\<close>, pre_expand)
+
+method str_tac = 
+  (match conclusion in "Q \<turnstile>\<^sub>p stabilize R True\<^sub>p" for Q R \<Rightarrow> \<open>succeed\<close>, rule stabilize_univ) |
+  (match conclusion in "Q \<turnstile>\<^sub>p stabilize R (str R P)" for Q R P \<Rightarrow> \<open>succeed\<close>, rule stabilize_str) |
+  (rule stabilize_trivial, solves \<open>stabilize_trivial_tac\<close>) 
+
+
+(*
+method solver =
+  (match conclusion in "Q \<turnstile>\<^sub>p chain R [] P" for Q R P \<Rightarrow> \<open>rule chain0, (simp )?\<close>) |
+  (match conclusion in "Q \<turnstile>\<^sub>p chain R xs P" for Q R xs P \<Rightarrow> 
+    \<open>rule chain1_full, solves \<open>pre_tac\<close>, solver\<close>) 
+*)
+
+named_theorems break
+
+lemma [break]: "stabilize R (P \<and>\<^sub>p Q) = (stabilize R P \<and>\<^sub>p stabilize R Q)"
+  unfolding stabilize_def by auto
+
+lemma [break]: "wpre a (P \<and>\<^sub>p Q) = (wpre a P \<and>\<^sub>p wpre a Q)"
+  by (cases a, auto)
+
+lemma [break]: "(P \<turnstile>\<^sub>p Q \<and>\<^sub>p Q') = ((P \<turnstile>\<^sub>p Q) \<and> (P \<turnstile>\<^sub>p Q'))"
+  by (auto simp: pred_defs)
+
+lemma [break]: "(P \<turnstile>\<^sub>p chain a (Q \<and>\<^sub>p Q')) = ((P \<turnstile>\<^sub>p chain a Q) \<and> (P \<turnstile>\<^sub>p chain a Q'))"
+  sorry
+
+declare wpre.simps [simp del]
+
+method breakdown = 
+  (simp add: wp_def break; intro conjI)
+
+method pre_expand = 
+  ((simp add: pre_defs guar_def
+        del: Orderings.order_top_class.top.extremum
+      split: iden.splits if_splits splits prod.splits)?; (rule subset_refl)?)
+
+method pre_str_tac =
+  (rule pre_str, solves \<open>pre_expand\<close>) | 
+  (rule pre_str_mod, pre_expand)
+
+method pre_tac =
+  (match conclusion in "Q \<subseteq> pre \<alpha> S UNIV" for \<alpha> S Q \<Rightarrow> \<open>succeed\<close>, rule pre_univ) |
+  (match conclusion in "Q \<subseteq> pre \<alpha> S (str R P)" for \<alpha> S Q R P \<Rightarrow> \<open>succeed\<close>, pre_str_tac) |
+  (match conclusion in "Q \<subseteq> pre \<alpha> S P" for Q \<alpha> S P \<Rightarrow> \<open>succeed\<close>, pre_expand)
+
+method solver =
+  (match conclusion in "Q \<turnstile>\<^sub>p chain [] P" for Q P \<Rightarrow> \<open>rule chain0, (rule str_mono)?, (simp only: trivial_thms)?\<close>) |
+  (match conclusion in "Q \<turnstile>\<^sub>p chain xs P" for Q xs P \<Rightarrow> 
+    \<open>rule chain1_full, solves \<open>str_tac\<close>, solves \<open>pre_tac\<close>, solver\<close>) 
+
+lemma ir_str:
+  "str R (wpre (ir r e) Q) \<turnstile>\<^sub>p wpre (ir r e) (str R Q)"
+  unfolding str_def pred_defs
+proof (clarsimp simp: wpre.simps)
+  fix m assume b: "stabilize R Q = Q" "stabilize R (\<lambda>m. Q (m(r :=\<^sub>r ev (rg m) e))) \<noteq>
+         (\<lambda>m. Q (m(r :=\<^sub>r ev (rg m) e)))"
+  hence a: "(\<lambda>m. \<forall>g. R (glb m, g) \<longrightarrow> Q (set_glb m g)) = Q" by (auto simp: stabilize_def)
+  have "(\<lambda>m. \<forall>g. R (glb m, g) \<longrightarrow> Q (set_glb m g)) o (\<lambda>m. m(r :=\<^sub>r ev (rg m) e)) = 
+         (\<lambda>m. Q (m(r :=\<^sub>r ev (rg m) e)))"
+    unfolding a by auto
+  hence "(\<lambda>m. \<forall>g. R (glb (m(r :=\<^sub>r ev (rg m) e)), g) \<longrightarrow> Q (set_glb (m(r :=\<^sub>r ev (rg m) e)) g)) = 
+         (\<lambda>m. Q (m(r :=\<^sub>r ev (rg m) e)))"
+    by (auto simp: o_def)
+  hence "stabilize R (\<lambda>m. Q (m(r :=\<^sub>r ev (rg m) e))) = (\<lambda>m. Q (m(r :=\<^sub>r ev (rg m) e)))"
+    unfolding stabilize_def
+    by (auto simp: set_glb_def rg_upd_def)
+  thus "Q (m(r :=\<^sub>r ev (rg m) e))" using b by simp
+qed
+
+lemma cm_str:
+  "str R (wpre (cm b) Q) \<turnstile>\<^sub>p wpre (cm b) (str R Q)"
+  unfolding str_def pred_defs
+proof (clarsimp simp: wpre.simps)
+  fix m assume b: "stabilize R Q = Q" "stabilize R (\<lambda>m. ev\<^sub>B (rg m) b \<longrightarrow> Q m) \<noteq>
+         (\<lambda>m. ev\<^sub>B (rg m) b \<longrightarrow> Q m)"
+  have "\<forall>m'. (\<lambda>m. \<forall>g. R (glb m, g) \<longrightarrow> Q (set_glb m g)) m' = Q m'" 
+    by (metis (full_types) b(1) stabilize_def) 
+  hence "\<forall>m. ((\<lambda>m. ev\<^sub>B (rg m) b) \<longrightarrow>\<^sub>p (\<lambda>m'. \<forall>g. R (glb m', g) \<longrightarrow> Q (set_glb m' g))) m = 
+         (\<lambda>m. ev\<^sub>B (rg m) b \<longrightarrow> Q m) m" by simp
+  hence "stabilize R (\<lambda>m. ev\<^sub>B (rg m) b \<longrightarrow> Q m) = (\<lambda>m. ev\<^sub>B (rg m) b \<longrightarrow> Q m)"
+    unfolding stabilize_def apply (auto simp: set_glb_def glb_def) 
+    by meson
+  thus "Q m" using b(2) by auto
+qed
+
+lemma st_str:
+  "\<forall>m m'. wpre (sr v x e a) Q m \<longrightarrow> R (glb m, glb m') \<longrightarrow> rg m' = rg m \<longrightarrow> wpre (sr v x e a) Q m' \<Longrightarrow>
+    str R (wpre (sr v x e a) Q) \<turnstile>\<^sub>p wpre (sr v x e a) (str R Q)"
+  unfolding str_def pred_defs
+  sorry
+
+lemma ld_str:
+  "\<forall>m m'. wpre (ld v x e a) Q m \<longrightarrow> R (glb m, glb m') \<longrightarrow> rg m' = rg m \<longrightarrow> wpre (ld v x e a) Q m' \<Longrightarrow>
+    str R (wpre (ld v x e a) Q) \<turnstile>\<^sub>p wpre (ld v x e a) (str R Q)"
+  unfolding str_def pred_defs
+  sorry
+
+
+lemma env_str:
+  "str R Q \<turnstile>\<^sub>p wpre (env R) (str R Q)"
+  sorry
+
+
+lemma chase_lev_put:
    "TOP = PTR \<Longrightarrow> BOT = PTR + 1 \<Longrightarrow> LEN = PTR + 2 \<Longrightarrow> BUF = PTR + 3 \<Longrightarrow> 
+    (\<forall>a b t. (a,b) \<in> S\<^sup>* \<longrightarrow> (a@t,b@t) \<in> S\<^sup>*) \<Longrightarrow>
     FNBEGIN
       R: =[BOT] \<and> \<le>[TOP] \<and> =[BUF] \<and> =[LEN] \<and> =[(BUF + (\<^sup>1[BOT] mod \<^sup>1[LEN]))] \<and> (\<^sup>1\<^sup>adeque,\<^sup>2\<^sup>adeque) \<in> S\<^sup>*
       G: \<le>[BOT] \<and> =[TOP] \<and> =[LEN]
       I: \<^sup>adeque = \<acute>(queue PTR) \<and> \<^sup>s[TOP] \<le> \<^sup>s[BOT]
       P: \<^sup>rr\<^sub>0 = PTR \<and> V = \<^sup>rr\<^sub>1 \<and> A = \<^sup>adeque \<and> SPACE = (\<^sup>s[BOT] - \<^sup>s[TOP] < \<^sup>s[LEN])
       {
-        r\<^sub>2 := [r\<^sub>0];
-        r\<^sub>3 := [r\<^sub>0 + #1];
+        \<lbrace> \<^sup>rr\<^sub>0 = PTR \<rbrace> r\<^sub>2 := [r\<^sub>0 + #0];
+        \<lbrace> \<^sup>rr\<^sub>0 = PTR \<rbrace> r\<^sub>3 := [r\<^sub>0 + #1];
         r\<^sub>2 := r\<^sub>3 - r\<^sub>2;
-        r\<^sub>4 := [r\<^sub>0 + #2];
+        \<lbrace> \<^sup>rr\<^sub>0 = PTR \<rbrace> r\<^sub>4 := [r\<^sub>0 + #2];
         if (LE r\<^sub>2 r\<^sub>4) then
           r\<^sub>2 := r\<^sub>3 % r\<^sub>4;
           r\<^sub>2 := r\<^sub>2 + r\<^sub>0;
@@ -102,27 +310,116 @@ lemma chase_lev_push:
       Q: SPACE \<longrightarrow> (A,\<^sup>adeque) \<in> S\<^sup>* O (put V) O S\<^sup>*
     FNEND" 
   apply (clarsimp simp add: local_props_def, intro conjI)
+  prefer 10
+
+  apply (simp add: break, intro conjI; simp only: append.simps chain_singleI' chain_singleI chain_lastI)
+
+  apply (rule chain1_full)
+  apply (blast)
+  apply (simp add: wpre.simps)
+  apply (simp add: break, intro conjI)
+  sorry
+
+  apply (rule chain1_full)
+  apply (simp add: wpre.simps)
+  apply (rule stabilize_trivial)
+  apply (auto simp: glb_def aux_upd_def o_def st_upd_def)[1]
+  apply (meson relcomp.relcompI transitive_closure_trans(3))
+
+  apply (rule chain1_full)
+  apply (rule ir_str)
+  apply (simp add: wpre.simps rg_upd_def addI_def)
+
+  apply (rule chain1_full)
+  apply (rule st_str)
+  apply (auto simp: glb_def aux_upd_def o_def st_upd_def wpre.simps)[1]
+  apply (meson relcomp.relcompI transitive_closure_trans(3))
+  apply (auto simp add: wpre.simps rg_upd_def st_upd_def aux_upd_def addI_def)[1]
+
+  apply (rule chain1_full)
+  apply (rule env_str)
+
+  apply (rule chain1_full)
+  apply (rule ir_str)
+  apply (simp add: wpre.simps rg_upd_def addI_def addR_def)
+
+  apply (rule chain1_full)
+  apply (rule ir_str)
+  apply (simp add: wpre.simps rg_upd_def addI_def modR_def)
+
+  apply (rule chain1_full)
+  apply (rule ir_str)
+  apply (simp add: wpre.simps rg_upd_def addI_def modR_def)
+
+  apply (rule chain1_full)
+  apply (rule cm_str)
+  apply (simp add: wpre.simps rg_upd_def addI_def modR_def LE_def)
+
+  apply (rule chain1_full)
+  apply (rule ld_str)
+  apply (auto simp: glb_def aux_upd_def rg_upd_def o_def st_upd_def wpre.simps)[1]
+  apply (meson relcomp.relcompI transitive_closure_trans(3))
+
+  apply (rule chain1_full)
+  apply (rule env_str)
+
+  apply (rule chain1_full)
+  apply (rule ir_str)
+  apply (simp add: wpre.simps rg_upd_def addI_def modR_def subR_def)
+  
+  apply (rule chain1_full)
+  apply (rule ld_str)
+  apply (auto simp: glb_def aux_upd_def rg_upd_def o_def st_upd_def wpre.simps)[1]
+  apply (meson relcomp.relcompI transitive_closure_trans(3))
+  
+  apply (rule chain1_full)
+  apply (rule env_str)
+
+  apply (rule chain1_full)
+  apply (rule ld_str)
+  apply (auto simp: glb_def aux_upd_def rg_upd_def o_def st_upd_def wpre.simps)[1]
+  apply (subgoal_tac "st m (Suc (rg m r\<^sub>0)) - st m (rg m r\<^sub>0) < st m (Suc (Suc (rg m r\<^sub>0)))")
+  apply auto[1]
+
+  defer 1
+  apply (meson relcomp.relcompI transitive_closure_trans(3))
+  apply (simp add: wpre.simps rg_upd_def addI_def modR_def subR_def)
+
+  apply (rule chain1_full)
+  apply (rule env_str)
+
+  apply (clarsimp simp add: chain.simps str_def pred_defs wpre.simps put_def split: if_splits)
+  
+  sorry
  
   (* Wellformedness *)
   apply (auto simp add: stable_def step\<^sub>t_def glb_def reflexive_def transitive_def)[4]
   apply (meson relcomp.relcompI rtrancl_trans)
 
   (* Various load operations *)
-  apply (auto simp: step_def wp_defs inv2_def)[3]
+  apply (auto simp: step_def wpre.simps wp_defs inv2_def)[3]
 
   (* Write to buffer *)
-  apply (auto simp: step_def st_upd_def glb_def aux_upd_def inv2_def set_glb_def wp_defs queue_def addI_def)[1]
+  apply (auto simp: step_def st_upd_def glb_def wpre.simps aux_upd_def inv2_def set_glb_def wp_defs entail_def queue_def addI_def)[1]
   apply (subgoal_tac "st m (Suc PTR) mod st m (Suc (Suc PTR)) \<noteq> x mod st m (Suc (Suc PTR))")
   apply argo
   apply (rule mod_neq; auto)
 
   (* Update BOT *)
-  apply (auto simp: step_def st_upd_def glb_def inv_def set_glb_def inv2_def aux_upd_def o_def wp_defs queue_def addI_def)[1]
-  apply (simp add: add.commute group_cancel.add1)  
+  apply (auto simp: step_def st_upd_def glb_def inv_def wpre.simps set_glb_def inv2_def aux_upd_def o_def entail_def wp_defs queue_def addI_def)[1]
   
+
   (* WP Reasoning *)  
   apply (clarsimp simp add: addR_def addI_def modR_def subR_def LE_def rg_upd_def)
   apply (clarsimp simp add: wp_defs rg_upd_def aux_upd_def st_upd_def)
+
+  apply (rule stabilize_rw)
+  apply (rule stabilize_rw)
+  apply (rule stabilize_rw)
+
+
+  sorry
+
   apply (clarsimp simp add: stabilize_def glb_def set_glb_def)
   apply safe
   apply auto
@@ -137,43 +434,40 @@ lemma chase_lev_push:
 
 lemma chase_lev_steal:
    "TOP = PTR \<Longrightarrow> BOT = PTR + 1 \<Longrightarrow> LEN = PTR + 2 \<Longrightarrow> BUF = PTR + 3 \<Longrightarrow> 
-    COBEGIN
+    FNBEGIN
       R: \<le>[TOP] \<and> =[LEN] \<and> (\<^sup>1\<^sup>adeque,\<^sup>2\<^sup>adeque) \<in> S\<^sup>*
       G: =[BOT] \<and> \<le>[TOP] \<and> =[LEN] \<and> (\<^sup>1[TOP] \<le> \<^sup>1[BOT] \<longrightarrow> \<^sup>2[TOP] \<le> \<^sup>2[BOT])
-      I: \<^sup>adeque = \<acute>(queue BASE)
-      P: \<^sup>rr\<^sub>0 = PTR \<and> V = \<^sup>rr\<^sub>1 \<and> A = \<^sup>adeque
+      I: \<^sup>adeque = \<acute>(queue PTR)
+      P: \<^sup>rr\<^sub>0 = PTR \<and> A = \<^sup>adeque
       {
-        r\<^sub>0 := #BASE;
-        r\<^sub>1 := [r\<^sub>0];
+        \<lbrace> \<^sup>rr\<^sub>0 = PTR \<rbrace> r\<^sub>1 := [r\<^sub>0 + #0];
         fence;
-        r\<^sub>2 := r\<^sub>0 + #1;
-        r\<^sub>2 := [r\<^sub>2];
+        \<lbrace> \<^sup>rr\<^sub>0 = PTR \<rbrace> r\<^sub>2 := [r\<^sub>0 + #1];
         if (LE r\<^sub>1 r\<^sub>2) 
         then
-          r\<^sub>2 := r\<^sub>0 + #2;
-          r\<^sub>2 := [r\<^sub>2];
+          \<lbrace> \<^sup>rr\<^sub>0 = PTR \<rbrace> r\<^sub>2 := [r\<^sub>0 + #2];
           r\<^sub>2 := r\<^sub>1 % r\<^sub>2;
-          r\<^sub>2 := r\<^sub>2 + #3;
           r\<^sub>2 := r\<^sub>2 + r\<^sub>0;
           cfence;
-          r\<^sub>2 := [r\<^sub>2];
+          \<lbrace> (\<exists>i. \<^sup>rr\<^sub>1 \<le> i \<and> i \<le> \<^sup>s[TOP] \<and> \<^sup>rr\<^sub>2 = PTR + (i mod \<^sup>s[LEN])) \<rbrace> 
+            r\<^sub>2 := [r\<^sub>2 + #3];
           r\<^sub>3 := r\<^sub>1 + #1;
-          (\<lbrace>\<^sup>rr\<^sub>3 = \<^sup>rr\<^sub>1 + 1 \<and> \<^sup>rr\<^sub>0 = TOP \<and> \<^sup>rr\<^sub>1 < \<^sup>s[BOT]\<rbrace> 
-            r\<^sub>3 := cas r\<^sub>0 r\<^sub>1 r\<^sub>3 , \<^sup>adeque := (case \<^sup>adeque of x#t \<Rightarrow> t));
-          if (Z r\<^sub>3) then r\<^sub>2 := #ABORT else Skip fi
+          \<lbrace> \<^sup>rr\<^sub>3 = \<^sup>rr\<^sub>1 + 1 \<and> \<^sup>rr\<^sub>0 = TOP \<and> \<^sup>rr\<^sub>1 < \<^sup>s[BOT] \<rbrace> 
+            r\<^sub>3 := cas r\<^sub>0 r\<^sub>1 r\<^sub>3, \<^sup>adeque := drop 1 \<^sup>adeque;
+          if (Z r\<^sub>3) then r\<^sub>2 := #ABORT fi
         else
           r\<^sub>2 := #EMPTY
         fi
       }
       Q: (\<^sup>rr\<^sub>2 \<noteq> EMPTY \<and> \<^sup>rr\<^sub>2 \<noteq> ABORT) \<longrightarrow> (A,\<^sup>adeque) \<in> S\<^sup>* O (steal \<^sup>rr\<^sub>2) O S\<^sup>*
-    COEND" 
+    FNEND" 
   sorry
 
 lemma chase_lev_take:
    "TOP = BASE \<Longrightarrow> BOT = BASE + 1 \<Longrightarrow> LEN = BASE + 2 \<Longrightarrow> BUF = BASE + 3 \<Longrightarrow> 
     COBEGIN
       R: =[BOT] \<and> \<le>[TOP] \<and> =[LEN]
-      G: \<le>[TOP] \<and> =[LEN] \<and> (\<^sup>1[TOP] \<le> \<^sup>1[BOT] \<longrightarrow> \<^sup>2[TOP] \<le> \<^sup>2[BOT])
+      G: \<le>[TOP] \<and> =[LEN]
       I: \<^sup>adeque = \<acute>(buffer BASE)
       P: True
       {
